

Chapter 2: Starting from the Natural Numbers

Definitions and Proofs

The Peano Axioms

Axiom 1

0 is a natural number.

Axiom 2

If N is a natural number, then $S(N)$ is also a natural number.

Axiom 3

0 is not the successor of any natural number.

$S(N) \neq 0$ for every natural number N .

Axiom 4

Different natural numbers must have different successors.

If N, M are natural numbers and $N \neq M$, then $S(N) \neq S(M)$. Equivalently, if $S(N) = S(M)$, then $N = M$.

Axiom 5 (Principle of Mathematical Induction)

Let $P(N)$ be any property pertaining to a natural number N . Suppose $P(0)$ is true, and suppose that whenever $P(N)$ is true, $P(S(N))$ is also true.

Then $P(N)$ is true for every natural number N .

Recursive Definition

Suppose for each natural number N , we have a function $f_n: N \rightarrow N$ from the natural numbers to the natural numbers. Let c be a natural number. Then we can assign a unique natural number a_n to each natural number N , such that $a_0 = c$ and $a_{s(N)} = f_n(a_n)$ for each natural number N .

Proof.

Using induction, prove base case, where $N = 0$.

Only 1 value of a_0 , which makes $a_0 = c$.

(None of the other definitions $a_{s(n)} = f_n(a_n)$ will redefine the value of a_0 , because of Axiom 3.

Thus, base case proven.

Suppose inductively that the procedure gives a single value to a_n . Then it gives a single value to $a_{s(n)} = f_n(a_n)$.

(None of the other definitions $a_{s(m)} = f_m(a_m)$ will redefine the value of $a_{s(n)}$, because of Axiom 4.

Induction completed. a_n is defined for each natural value n , with a single value assigned to each a_n .

□

Definition: Addition of Natural Numbers

Addition is a function that maps two natural numbers (two elements of N) to another one. It is defined recursively as:

$$0 + m := m \rightarrow (1)$$

$$S(N) + m := S(N + m) \rightarrow (2)$$

Example:

$$0 + m = m \quad (\text{Definition 1})$$

$$\begin{aligned} 1 + m &= S(0) + m \\ &= S(0 + m) \quad (\text{Definition 2}) \\ &= S(m) \quad (\text{Definition 1}) \end{aligned}$$

$$\begin{aligned} 2 + m &= S(1) + m \\ &= S(1 + m) \quad (\text{Definition 2}) \\ &= S(m) \end{aligned}$$

Definition: Positive Natural Numbers

A natural number N is said to be positive if and only if it is not equal to zero.

Definition: Ordering of Natural Numbers

Let N and M be natural numbers.

$N \sqsubseteq M$ or $M \leq N$ if and only if $N = M + a$ for some natural number a .

N is strictly greater than M , $N > M$ or $M > N$ if and only if $N \sqsubseteq M$ and $N \neq M$

$S(N) > N$ for any N , thus there is no largest natural number N .

Definition: Multiplication of Natural Numbers

Multiplication is a function mapping two natural numbers to another one. It is defined recursively as:

$$0 \times m := 0 \rightarrow (1)$$

$$S(N) \times m := (N \times m) + m \rightarrow (2)$$

Example:

$$0 \times m = 0 \quad (\text{by definition 1})$$

$$1 \times m = S(0) \times m = (0 \times m) + m = m \quad (\text{by definition 2})$$

Definition: Exponentiation of Natural Numbers

Let m be a natural number. To raise m to the power 0, we define $m^0 := 1$; in particular, we define $0^0 := 1$. Now suppose recursively that m^n has been defined for some natural number n , then we define $m^{s(n)} := m^n \times m$

Proposition 1: 3 is a natural number

Proof.

0 is a natural number. (Axiom 1)

$S(0) = 1$ is a natural number. (Axiom 2)

$S(1) = 2$ is also a natural number. (Axiom 2)

Hence, $S(2) = 3$ is a natural number. (Axiom 2)

Proposition 2: 4 is not equal to 0.

Proof.

By definition, $4 = S(3)$.

3 is a natural number. (Axiom 1 and 2, or Proposition 1)

$S(3) \neq 0$ (Axiom 3)

Hence, $4 \neq 0$.

Proposition 3: 6 is not equal to 2.

Proof by contradiction.

Suppose $6 = 2$. Then $S(5) = S(1)$, which leads to $5 = 1$. (Axiom 4)

$S(4) = S(0)$

Then, $4 = 0$ (Axiom 4)

This contradicts Proposition 2.

Proposition 4: A certain property $P(N)$ is true for every natural number N .

Using the Principle of Mathematical Induction (Axiom 5),

1. Verify base case, where $N = 0$
Prove $P(0)$.
2. Suppose inductively that $P(N)$ is true for every natural number N .
 $P(N)$ is proven.
3. Prove for $P(S(N))$.
Insert proof here, assuming $P(N)$ is true.

Closes induction, thus $P(N)$ is true for every natural number N .

Proposition 5: The sum of two natural numbers is a natural number.

Proof.

Induct on m , keeping n fixed.

Let N be a natural number, $M + N$ is a natural number.

Proving base case, $M = 0$.

$0 + N = N$ (Addition Definition)

Since N is a natural number, the base case is proven.

Induction Step:

Suppose M is a natural number, $M + N$ is a natural number.

Prove $S(M) + N$ is a natural number.

$S(M) + N = S(M + N)$ (Addition Definition)

Since $M + N$ is a natural number (Induction Step)

$S(M + N)$ is also a natural number. (Axiom 2)

Lemma 6: For any natural number M , $M + 0 = M$.

Proof.

Prove base case, $M = 0$.

$0 + 0 = 0$ (Addition Definition 1: $0 + M = M$)

Base case is proven.

Induction case:

Suppose $M + 0 = M$

Prove $S(M) + 0 = S(M)$.

$S(M) + 0$

$= S(M + 0)$ (Addition Definition 2)

$= S(M)$ (Induction Step)

Lemma 7: For any natural numbers N and M , $N + S(M) := S(N + M)$

Proof.

Induction on N , keeping M fixed.

Base case, $N = 0$.

$0 + S(M)$

$= S(0 + M)$ (Addition Definition 2)

$= S(M)$ (Addition Definition 1)

Base Case is proven.

Induction case:

Suppose $N + S(M) := S(N + M)$.

Prove $S(N) + S(M) = S(S(N) + M)$.

LHS: $S(N) + S(M)$

$= S(N + S(M))$ (Addition Definition 2)

$= S(S(N + M))$ (Induction Case)

RHS: $S(S(N) + M)$

$= S(S(N + M))$ (Addition Definition 2)

Close induction.

Proposition 8: (Addition is Commutative) For any natural numbers N and M , $N + M = M + N$

Proof.

Induction on N , keeping M fixed.

Base case, $N = 0$.

LHS: $0 + M = M$ (Addition Definition 1)

RHS: $M + 0 = M$ (Lemma 6)

Hence, the base case is proven.

Induction Case:

Suppose $N + M = M + N$

Prove $S(N) + M = M + S(N)$

LHS: $S(N) + M$

$= S(N + M)$ (Addition Definition 2)

RHS: $M + S(N)$

$= S(M + N)$ (Lemma 7)

$= S(N + M)$ (Induction Step)

Close induction.

Proposition 9: (Addition is Associative) For any natural numbers A, B, C , $(A + B) + C = A + (B + C)$

Proof.

Induction on A , keeping B and C fixed.

Prove base case, $A = 0$

$(0 + B) + C = 0 + (B + C)$

LHS: $(0 + B) + C$

$= B + C$ (Addition Definition 1: $0 + M = M$)

RHS: $0 + (B + C)$

$= B + C$ (Addition Definition 1: $0 + M = M$)

Hence, $(0 + B) + C = 0 + (B + C)$ as required.

Induction Step:

Suppose $(A + B) + C = A + (B + C)$

Prove $(S(A) + B) + C = S(A) + (B + C)$

LHS: $(S(A) + B) + C$

$= S(A + B) + C$ (Addition Definition 2)

$= S(A + B + C)$ (Addition Definition 2)

RHS: $S(A) + (B + C)$

$$= S(A + B + C) \text{ (Addition Definition 2)}$$

Close induction.

Proposition 10: Cancellation Law. Let natural numbers A, B, C such that $A + B = A + C$, implies $B = C$

Proof.

Induction on A , keeping B and C fixed.

Prove base case, $A = 0$

$$0 + B = 0 + C$$

$$B = C \text{ (Addition Definition 1)}$$

Induction Step:

Suppose $A + B = A + C$, implies $B = C$

Prove $S(A) + B = S(A) + C$, implies $B = C$

$$S(A + B) = S(A + C) \text{ (Addition Definition 2)}$$

$$A + B = A + C \text{ (Axiom 4)}$$

$B = C$ is implied. (Induction Step)

Proposition 11: If A is positive and B is a natural number, then $A + B$ is positive (and hence so is $B + A$)

Proof.

Induction on B , keeping A fixed.

Prove base case, $B = 0$

$$A + B = A + 0 = A \text{ (Lemma 6)}$$

Since A is positive, the base case is proven.

Induction Step:

Suppose $A + B$ is positive

Prove $A + S(B)$ is positive.

$$A + S(B) = S(A + B) \text{ (Lemma 7)}$$

Since $S(A + B) \neq 0$ (Axiom 3), and $S(A + B)$ is a natural number (Axiom 2), hence $S(A + B)$ is positive.
(Definition of Positive Numbers)

Corollary 12: If A and B are natural numbers such that $A + B = 0$, then $A = 0$ and $B = 0$.

Proof by Contradiction.

Suppose $A \neq 0$ or $B \neq 0$.

$A \neq 0$ shows that A is positive (Definition of Positive Numbers)

Hence, $A + B = 0$ is positive (Proposition 11).

Contradicts the Definition of Positive Numbers.

$B \neq 0$ then B is positive.

Hence, $A + B = 0$ is positive (Proposition 11).

Contradicts the Definition of Positive Numbers.

Therefore, $A = 0$ and $B = 0$

Lemma 13: Let A be a positive number. Then there exists exactly one natural number B such that $S(B) = A$.

Proof.

Prove the base case, $B = 0$.

$S(0) = 1$

0 is a natural number. (Axiom 1)

1 is also a natural number. (Axiom 2)

There can only be one unique successor for 0, which is 1. (Axiom 4)

Since 1 is also a positive number, the base case is proven.

Induction case: There exists exactly one natural number B such that $S(B)$ is a positive number.

Prove $S(S(B))$ is positive.

$S(B)$ is positive (Induction case).

$S(B)$ is natural. (Axiom 2)

$S(S(B))$ is also natural. (Axiom 2)

$S(S(B))$ is not zero. (Axiom 3)

Hence, $S(S(B))$ is positive. (Definition of Positive Numbers)

Proposition 14: (Basic Properties of Order for Natural Numbers)

Let A , B and C be natural numbers. Then

- a. Order is reflexive. $A \leq A$.

Proof.

Since $A \leq A$, $A = A + n$ for some natural number n (Definition of Order)

Let $n = 0$,

$A + n$ (0 is a natural number, Axiom 1)

$= A + 0$ (Lemma 6)

$= A$

Hence, $A \leq A$ as required.

- b. Order is transitive. If $A \sqsubseteq B$ and $B \sqsubseteq C$, then $A \sqsubseteq C$.

Proof.

$A \sqsubseteq B$ and $B \sqsubseteq C$ for some natural numbers n and m . (Definition of Order)

Hence, $A \sqsubseteq C + (m + n)$. (Definition of Order)

Therefore, $A \sqsubseteq C$.

- c. Order is antisymmetric. If $A \sqsubseteq B$ and $B \sqsubseteq A$, then $A = B$.

Proof.

$A \sqsubseteq B$ implies $A = B + n$

$B \sqsubseteq A$ implies $B = A + m$

$A = (A + m) + n$

$A = A + (m + n)$ (Associative Law)

$m + n$ is zero for the previous statement to be true. (Definition of Addition)

$m + n = 0$

Hence, $m = 0$ and $n = 0$ (Corollary 12)

As such, $A = B$.

- d. (Addition preserves order) $A \sqsubseteq B$ if and only if $A + C \sqsubseteq B + C$

$A + C \sqsubseteq B + C$

$A + C = B + C + m$

$A = B + m$

Hence, $A \sqsubseteq B$ if and only if $A + C \sqsubseteq B + C$.

$A \sqsubseteq B$

$A = B + m$

$B + m + C \sqsubseteq B + C$

Hence, true by definition and $A + C \sqsubseteq B + C$ if and only if $A \sqsubseteq B$.

- e. $A < B$ if and only if $S(A) \leq B$

$A < B$ implies that $B = A + d$, where $d > 0$. (Definition of Order)

$B = A + S(C)$

$B = S(A + C)$

$S(A + C) \sqsubseteq S(A)$

$B \sqsubseteq S(A)$

$S(A) \leq B$

- f. $A < B$ if and only if $B = A + d$ for some positive number d .

$A < B$ implies that $B = A + d$, where $d > 0$. (Definition of Order)
Since $d > 0$, d is positive. (Definition of Positive Numbers)

or

$B = A + d$, then $B \neq A$

Prove $B \neq A$.

Suppose for contradiction $B = A$, then by cancellation, $d = 0$.

Which means d is not positive, thus a contradiction.

Proposition 15: (Trichotomy of Order of Natural Numbers)

Let A and B be natural numbers. Then exactly one of the following statements is true: $A < B$, $A = B$, $B < A$.

Proof.

No more than one of the statements can hold true at the same time.

If $A < B$, then $A \neq B$.

If $B < A$, then $A \neq B$.

However, if $A < B$ and $B < A$, then $A = B$. (Proposition 14).

Hence, a contradiction with the two earlier statements.

One of the statements is true.

Induction on A , keep B fixed.

Base case:

When $A = 0$,

$0 \leq B$

Since B is a natural number, B might be zero. (Axiom 1)

So either $0 = B$ or $0 < B$.

The base case is proven.

Suppose $A < B$, $A = B$, $B < A$.

Prove $S(A)$ for each statement.

$B < A$, then $B < S(A)$

$A = B + d$

$d = S(c)$ for some natural number c

$A = B + S(c)$

$A = S(B + c)$ (Definition of Addition)

$S(A) = S(S(B + c))$ (Axiom 4)

$B < S(S(B + c))$

If $A = B$, then $S(A) > B$.

$S(A) = S(B)$ (Axiom 4)

$S(B) > B$

If $A < B$,
 $S(A) \leq B$ (Proposition 14e)
 Then either $S(A) = B$ or $S(A) < B$.

Close induction.

Proposition 16 (Strong Principle of Induction)

Let m_0 be a natural number, and let $P(m)$ be a property pertaining to an arbitrary natural number m . Suppose that for each $m \geq m_0$, we have the following implication: if $P(m)$ is true for all natural numbers $m_0 \leq m < m$, then $P(m)$ is also true. (In particular, this means that $P(m_0)$ is true, since in this case the hypothesis is vacuous.) Then we can conclude that $P(m)$ is true for all natural numbers $m \geq m_0$.

Hints: Define $Q(n)$ to be the property that $P(m)$ is true for all $m_0 \leq m < n$; note that $Q(n)$ is vacuously true when $n < m_0$.

Proof.

Let $Q(n)$ be the property that $P(m)$ is true for all $m_0 \leq m < n$. Given this definition of Q , we can restate the hypothesis for P as follows: for each $m \geq m_0$, if $Q(m)$ is true then $P(m)$ is also true. We will prove by induction that $Q(n)$ is true for all natural numbers n .

We first want to show $Q(0)$, which says that $P(m)$ is true for all $m_0 \leq m < 0$. This is vacuously true since there is no natural number strictly less than zero: $m < 0$ means $m \leq 0$ and $m \neq 0$. So we have some natural number a such that $0 = m + a$, but this means $m = 0$ by Corollary 2.2.9, which contradicts the fact that $m \neq 0$. So $P(m)$ is true for all such numbers, because none exist.

Now suppose inductively that we have shown $Q(n)$ is true. We want to show that $Q(S(n))$ is true, i.e. we want to show that $P(m)$ is true for all $m_0 \leq m < S(n)$. So let m be a natural number and suppose $m_0 \leq m < S(n)$. Our goal is to show that $P(m)$ is true.

Since $m_0 \leq m < S(n)$, we claim that either $m_0 \leq m < n$ or $m = n$. This is because $m < S(n)$ implies $S(m) \leq S(n)$ by Proposition 2.2.12(e) which implies $m \leq n$ by Proposition 2.2.12(d). We know $m = n$ or $m \neq n$; in the latter case we thus have $m < n$, so $m_0 \leq m < n$. Thus we see that either $m_0 \leq m < n$ or $m = n$.

Since $Q(n)$ is true, we know that $P(m)$ is true for all $m_0 \leq m < n$. Thus in the case where $m_0 \leq m < n$, we already know that $P(m)$ is true

To complete the proof we must show that $P(m)$ is true in the case $m = n$, i.e. we must show that $P(n)$ is true. Since $m_0 \leq m < S(n)$, by transitivity of order $m_0 < S(n)$, so $m_0 \leq S(n)$ which means $m_0 \leq n$. Since $m_0 \leq n$, we can use the hypothesis for P , which says that if $Q(n)$ is true then $P(n)$ is also true. Since $Q(n)$ is true by inductive hypothesis, we see that $P(n)$ is true as desired.

This completes the induction, and we have that $Q(n)$ is true for all natural numbers n . Our original goal was to show that $P(m)$ is true for all natural numbers $m \geq m_0$. So let $m \geq m_0$. Then we know that $Q(S(m))$ is true. Since $m_0 \leq m < S(m)$, we see that $P(m)$ is true as required.

Source: <https://taoanalysis.wordpress.com/2020/04/01/exercise-2-2-5/>

Proposition 17: Principles of Backwards Induction

Let n be a natural number, and let $P(m)$ be a property pertaining to the natural numbers such that whenever $P(m++)$ is true, then $P(m)$ is true. Suppose that $P(n)$ is also true. Prove that $P(m)$ is true for all natural numbers $m \leq n$; this is known as the principle of backwards induction.

Hint:

Apply induction to the variable n .

For the statement to prove via induction, use the following: if $P(n)$ is true, then $P(m)$ is true for all $m \leq n$.

Let P be a property pertaining to the natural numbers such that whenever $P(S(m))$ is true, $P(m)$ is true.

Let $Q(n)$ be the following statement: if $P(n)$ is true, then $P(m)$ is true for all $m \leq n$.

We shall show that $Q(n)$ is true for all n using induction. For the base case, we must show $Q(0)$. So suppose that $P(0)$ is true. We want to show that $P(m)$ is true for all $m \leq 0$. By definition of inequality (definition 2.2.11), $m \leq 0$ means that $0 = m + a$ for some natural number a . By corollary 2.2.9, we have $m = 0$. In other words, $m \leq 0$ implies $m = 0$, so showing that $P(m)$ for all $m \leq 0$ is equivalent to showing $P(0)$, which we already know. This completes the base case.

Now suppose $Q(n)$ is true. We must show that $Q(S(n))$ is true. So suppose that $P(S(n))$ is true. We need to show that $P(m)$ is true for all $m \leq S(n)$. We know that whenever $P(S(m))$ is true, $P(m)$ is true, so for $m = n$ in particular this means that if $P(S(n))$ is true then $P(n)$ is true. Since $P(S(n))$ is true, we see that $P(n)$ is true. By the induction hypothesis we thus have $P(m)$ for all $m \leq n$. Now let $m \leq S(n)$. We want to show that $P(m)$ is true. If we can show that $m \leq n$ or $m = S(n)$, then we will be done, because in either case we have already shown that $P(m)$ is true. To show that $m \leq n$ or $m = S(n)$, we will show that $m \neq S(n)$ implies $m \leq n$. Suppose $m \neq S(n)$. This means $m < S(n)$ by definition 2.2.11. By proposition 2.2.12(e), we have $S(m) \leq S(n)$, i.e. $m + 1 \leq n + 1$. By proposition 2.2.12(d) this means $m \leq n$ as required. This closes the induction.

Now let n be a natural number, and suppose $P(n)$ is true. By our work above, we know that $Q(n)$ is true. This means that $P(m)$ is true for all natural numbers $m \leq n$ as required.

Source: <https://taoanalysis.wordpress.com/2020/03/16/exercise-2-2-6/>

Proposition 18: (Multiplication is commutative). Let N, M be natural numbers. Then $N \times M = M \times N$.

Prove $0 \times M = M \times 0$

Base case: $M = 0$

LHS: $0 \times 0 = 0$ (Multiplication Definition 1)

RHS: $0 \times 0 = 0$

The base case is proven.

Induction case:

Assume $0 \times M = M \times 0$

Prove for $S(M)$

$$0 \times S(M) = S(M) \times 0$$

LHS: $0 \times S(M) = 0$ (Multiplication Definition 1)

RHS: $S(M) \times 0 = (M \times 0) + 0 = 0 + 0 = 0$ (Multiplication Definition 2, Induction Case)

Close induction. Proven that $0 \times M = M \times 0$

Prove that $M \times S(N) = (M \times N) + M$

Induction on M , keep N fixed.

Base case: $M = 0$

$$0 \times S(N) = (0 \times N) + 0$$

LHS: $0 \times S(N) = 0$ (Multiplication Definition 1)

RHS: $(0 \times N) + 0 = 0$

Base case is proven.

Assume that $M \times S(N) = (M \times N) + M$

Prove for $S(M)$

$$S(M) \times S(N) = (S(M) \times N) + S(M)$$

LHS: $S(M) \times S(N)$

$= (M \times S(N)) + S(M)$ (Multiplication Definition 2)

$= ((M \times N) + M) + S(M)$ (Induction Case)

$= (M \times N) + M + S(M)$

RHS: $(S(M) \times N) + S(M)$

$= (N \times M) + M + S(M)$ (Multiplication Definition 2)

Close induction. Proven that $M \times S(N) = (M \times N) + M$

Proof.

Induction on N , keep M fixed.

Base case when $N = 0$.

LHS: $0 \times M = 0$ (Multiplication Definition 1)

RHS: $M \times 0 = 0$ (Proven earlier)

Induction Case:

Assume $N \times M = M \times N$

Prove for $S(N)$

LHS: $S(N) \times M = (N \times M) + M$ (Multiplication Definition 2)

RHS: $M \times S(N)$

$$= (M \times N) + M \text{ (Proven earlier)}$$

$$= (N \times M) + M \text{ (Induction case)}$$

Close induction. Proven that $N \times M = M \times N$

Lemma 19: (Positive natural numbers have no zero divisors). Let n, m be natural numbers. Then $n \times m = 0$ if and only if at least one of n, m is equal to zero. In particular, if n and m are both positive, then nm is also positive.

Proof by Contradiction.

Assuming that $n \neq 0$ and $m \neq 0$, n and m are both positive. (Definition of Natural Numbers)

$$n = S(p) \text{ so } n \times m = S(p) \times m = (p \times m) + m = 0$$

So, $(p \times m) = 0$ and $m = 0$ (Corollary 12)

Contradiction since m is positive (Definition of Natural Numbers)

So at least one of n, m is equal to zero.

Prove that at least one of n, m is equal to zero, then $n \times m = 0$.

If $m = 0$, then $n \times 0 = 0$ (Commutative Law)

If $n = 0$, then $0 \times m = 0$ (Multiplication Definition 1)

Prove that the multiplication of natural numbers n and m is also a natural number.

Base case, $n = 0$.

$$0 \times m = 0$$

Thus, the base case is proven.

Assume multiplication of natural numbers n and m is also a natural number.

Since $n = S(p)$ so $n \times m = S(p) \times m = (p \times m) + m$ is a natural number, since $(p \times m)$ is a natural number. (Induction case)

Prove that if n and m are both positive, then nm is also positive.

nm is a natural number, so let $nm = 0$.

As proven earlier, at least one of n, m is equal to zero, then $n \times m = 0$.

But n and m are both positive, thus a contradiction.

Proposition 20: (Distributive law). For any natural numbers a, b, c , we have $a(b + c) = ab + ac$ and $(b + c)a = ba + ca$.

Proof.

Since multiplication is commutative, show only the first statement.

Prove base case, $c = 0$.

$$\text{LHS: } a(b + 0) = ab$$

$$\text{RHS: } ab + a0 = ab + 0 = ab$$

The base case is proven.

Assume that $a(b + c) = ab + ac$

Proven for $S(c)$

LHS: $a(b + S(c)) = a(S(b+c)) = a(b + c) + a = ab + ac + a$

RHS: $ab + aS(c) = ab + a(c+1) = ab + ac + a$

Proposition 21: (Multiplication is associative). For any natural numbers a, b, c , we have $(a \times b) \times c = a \times (b \times c)$.

Proof.

Prove base case, $c = 0$.

LHS: $(a \times b) \times 0 = a \times b$ (Proven earlier)

RHS: $a \times (b \times 0) = a \times 0 = a$ (Multiplication Definition)

Proposition 22: (Multiplication preserves order). If a, b are natural numbers such that $a < b$, and c is positive, then $ac < bc$.

Proof.

Since $a < b$, then $b = a + d$ for some positive d .

Multiply both sides by c , $bc = ac + dc$

Since d and c are both positive, then dc is also positive. (Lemma 19)

So $ac < bc$ as desired.

Corollary 23: (Cancellation law). Let a, b, c be natural numbers such that $ac = bc$ and c is non-zero. Then $a = b$.

Proof.

By the trichotomy of order, (Proposition 15) $A < B$ and $B < A$, then $A = B$.

Suppose that $A > B$, then $AC > BC$, hence a contradiction. (Proposition 22)

Suppose that $A < B$, then $AC < BC$, hence a contradiction.

$A = B$ is the only possibility.

Proposition 2.3.9 (Euclidean algorithm). Let n be a natural number, and let q be a positive number. Then there exist natural numbers m, r such that $0 \leq r < q$ and $n = mq + r$.

Proof.

Fix q and induct on n .

Prove the base case, $n = 0$.

$0 = mq + r$

Hence, r and m are 0, (Corollary 12)

So $0 \leq 0 < q$ which is true.

Now suppose inductively that there are natural numbers m, r such that $0 \leq r < q$ and $n = mq + r$.

We must show that there are natural numbers m', r' such that $0 \leq r' < q$ and $n + 1 = m'q + r'$.

We have two cases, $r + 1 = q$ and $r + 1 \neq q$. If $r + 1 = q$, we can take $m' := m + 1$ and $r' := 0$. Then $0 \leq r' = 0 < q$ and we have $m'q + r'$ equal to $(m+1)q + 0$ by definition of m', r' , which equals $mq + q$ by the distributive law, which equals $mq + r + 1$ by using $q = r + 1$, which equals $n + 1$ by the inductive hypothesis $n = mq + r$. Thus $m'q + r' = n + 1$ as required.

Now suppose $r + 1 \neq q$. In this case, $r < q$ from the inductive hypothesis gives $r + 1 \leq q$, so $r + 1 < q$. So we can take $r' := r + 1$ and $m' := m$. Now $0 \leq r' < q$ by what we just showed, and $m'q + r' = mq + r + 1 = n + 1$ by definition of m', r' and the inductive hypothesis $n = mq + r$.

Exercise 2.3.4. Prove the identity $(a + b)^2 = a^2 + 2ab + b^2$ for all natural numbers a, b .

Proof.

$$(a + b)^2 = (a + b)^1(a + b) = (a + b)(a + b) \text{ (Definition of Exponentiation)}$$

$$(a + b)(a + b)$$

$$= a(a + b) + b(a + b) \text{ (Distributivity Law)}$$

$$= aa + ab + ba + bb \text{ (Commutative Law)}$$

$$= a^2 + ab + ab + b^2 \text{ (Definition of Exponentiation)}$$

Show that $ab + ab = 2ab$

$$2ab = 2 \times ab = (1 \times ab) + ab = ab + ab$$

$$= a^2 + 2ab + b^2$$